src/Zulib/fstar/Zen.Cost.Extracted.fst
@@ -3,19 +3,19 @@ module Zen.Cost.Extracted
 open Zen.Base
 open Zen.Cost.Realized
 
-val refine_prop_in(#a:Type)(#n:nat):
+val refine_in(#a:Type)(#n:nat):
     p:(a -> prop)
     -> mx:cost a n{p (force mx)}
     -> cost (x:a{p x}) n
-let refine_prop_in #a #n p mx =
+let refine_in #a #n p mx =
     force_prop p;
     retype (cost (x:a{p x}) n) mx
 
-val refine_prop_out(#a:Type)(#n:nat):
+val refine_out(#a:Type)(#n:nat):
     p:(a -> prop)
     -> cost (x:a{p x}) n
     -> mx:cost a n{p (force mx)}
-let refine_prop_out #a #n p mx =
+let refine_out #a #n p mx =
     force_prop p;
     retype (mx:cost a n{p (force mx)}) mx
 
@@ -23,14 +23,14 @@ val refine_eq_in(#a:Type)(#n:nat):
     mx:cost a n
     -> cost (x:a{x == force mx}) n
 let refine_eq_in #_ #_ mx =
-    refine_prop_in (fun x -> x == force (mx)) mx
+    refine_in (fun x -> x == force (mx)) mx
 
 val refine_eq_out(#a:Type)(#n:nat):
     x:a ->
     cost (y:a{y==x}) n
     -> mx:cost a n{force mx == x}
 let refine_eq_out #_ #_ x mx =
-    refine_prop_out (fun y -> y == x) mx
+    refine_out (fun y -> y == x) mx
 
 val incRet(#a:Type): n:nat -> a -> cost a n
 let incRet(#_) n x = inc n (ret x)
