src/Zulib/fstar/Zen.Cost.Realized.fst
@@ -29,6 +29,12 @@ abstract let bind #_ #_ #_ #_ (C x) f = C (C?.inj (f x))
 abstract val inc(#a:Type)(#n: nat): k:nat -> cost a n -> cost a (n+k)
 abstract let inc #_ #_ k (C x) = C x
 
+//
+// Escape: Cannot be used in programs due to Ghost effect
+//
+
+abstract val force(#a:Type)(#n:nat): cost a n -> GTot a
+abstract let force #_ #_ (C x) = x
 
 //
 // Monad Laws
@@ -45,11 +51,15 @@ val assoc(#a #b #c:Type)(#n1 #n2 #n3:nat):
   -> Lemma ((m `bind` f) `bind` g == m `bind` (fun x -> f x `bind` g))
 let assoc #_ #_ #_ #_ #_ #_ _ _ _ = ()
 
+//
+// Lemmas about force
+//
 
-// These functions are intentionally not implemented. They cannot be used in actual code.
-// Nevertheless, they are very useful for theorem proving.
-abstract val force(#a:Type)(#n:nat): cost a n -> GTot a
-abstract let force #_ #_ mx = C?.inj mx
+// This can't be proven due to polarity on `C` ie. `C #a =!= C #(x:a{p x})`.
+// Since `C` is not exposed, this is irrelevant, so we can assume this lemma.
+assume val force_prop(#a:Type):
+    p:(a -> prop)
+    -> Lemma (forall (n:nat). cost (x:a{p x}) n == mx:cost a n{p (force mx)})
 
 val force_ret(#a:Type): x:a -> Lemma (force (ret x) == x)
                                [SMTPat (ret x)]
@@ -58,17 +68,12 @@ val force_inc(#a:Type)(#m:nat):
   n:nat -> mx: cost a m -> Lemma(force (inc n mx) == force mx)
                            [SMTPat (inc n mx)]
 let force_inc #_ #_ _ _ = ()
-val force_bind(#a #b:Type)(#m #n:nat): mx:cost a m -> f:(a -> cost b n)
-  -> Lemma(force (f (force mx)) == force (bind mx f))
-     [SMTPat (bind mx f)]
+val force_bind(#a #b:Type)(#m #n:nat):
+    mx: cost a m
+    -> f:(a -> cost b n)
+    -> Lemma(force (f (force mx)) == force (bind mx f))
+       [SMTPat (bind mx f)]
 let force_bind #_ #_ #_ #_ _ _ = ()
-
-val refine: a:Type u#t -> p:(a -> prop) -> Type u#t
-let refine a p = x:a{p x}
-
-assume val force_prop(#a:Type):
-    p:(a -> prop)
-    -> Lemma (forall (n:nat). cost (x:a{p x}) n == mx:cost a n{p (force mx)})
 
 val force_bind_inc(#a #b:Type)(#m #n:nat):
     mx:cost a m
